examples/dynamic_isolation/External.v
@@ -3,15 +3,16 @@ Require Import Koika.Std.
 
 Require Import DynamicIsolation.Interfaces.
 
-Module External <: External_sig.
+Module OriginalExternal <: External_sig.
   Import Common.
-  Inductive memory := imem | dmem | mainmem.
+  Inductive memory := imem | dmem.
 
   Inductive ext_fn_t' :=
   | ext_mem (m: memory)
   | ext_uart_read
   | ext_uart_write
-  | ext_led.
+  | ext_led
+  .
 
   Definition ext_fn_t := ext_fn_t'.
   Definition led_input := maybe (bits_t 1).
@@ -21,6 +22,91 @@ Module External <: External_sig.
   Definition Sigma (fn: ext_fn_t) :=
     match fn with
     | ext_mem _ => {$ struct_t mem_input ~> struct_t mem_output $}
+    | ext_uart_read => {$ bits_t 1 ~> uart_output $}
+    | ext_uart_write => {$ uart_input ~> bits_t 1 $}
+    | ext_led => {$ led_input ~> bits_t 1 $}
+    end.
+
+  Definition ext_fn_specs (fn: ext_fn_t) :=
+    match fn with
+    | ext_mem imem => {| ef_name := "ext_mem_imem"; ef_internal := false |}
+    | ext_mem dmem => {| ef_name := "ext_mem_dmem"; ef_internal := false |}
+    | ext_uart_write => {| ef_name := "ext_uart_write"; ef_internal := false |}
+    | ext_uart_read => {| ef_name := "ext_uart_read"; ef_internal := false |}
+    | ext_led => {| ef_name := "ext_led"; ef_internal := false |}
+    end.
+
+  Instance Show_ext_fn_t : Show ext_fn_t := _.
+
+End OriginalExternal.
+
+
+Module External <: External_sig.
+  Import Common.
+  Inductive memory := imem | dmem | mainmem.
+
+  Inductive ext_fn_t' :=
+  | ext_mem (m: memory)
+  | ext_uart_read
+  | ext_uart_write
+  | ext_led
+  .
+
+
+  Definition ext_fn_t := ext_fn_t'.
+  Definition led_input := maybe (bits_t 1).
+  Definition uart_input := maybe (bits_t 8).
+  Definition uart_output := maybe (bits_t 8).
+
+  Definition log_num_sets := 12.
+  Definition log_tag_size := 18. (* 32 - 2 - 12 *)
+
+  Definition cache_tag_t := bits_t log_tag_size. (* TODO  *)
+  Definition cache_index_t := bits_t log_num_sets.
+  (* TODO: avoiding Koika arrays for now. This should be an array based on the block size *)
+  Definition cache_line_t := bits_t 32.
+
+  Definition MSI :=
+    {| enum_name := "MSI";
+       enum_members := vect_of_list ["M"; "S"; "I"];
+       enum_bitpatterns := vect_of_list [Ob~0~0; Ob~0~1; Ob~1~0] |}.
+
+  Definition ext_cache_mem_req :=
+    {| struct_name := "ext_cache_mem_req";
+       struct_fields := [("byte_en", bits_t 4);
+                         ("tag", cache_tag_t);
+                         ("index", cache_index_t);
+                         ("data", bits_t 32);
+                         ("MSI", maybe (enum_t MSI))] |}.
+
+  Definition cache_mem_input :=
+    {| struct_name := "cache_mem_input";
+       struct_fields := [("get_ready", bits_t 1);
+                         ("put_valid", bits_t 1);
+                         ("put_request", struct_t ext_cache_mem_req)] |}.
+
+  Definition cache_row :=
+    {| struct_name := "cache_row";
+       struct_fields := [("tag", cache_tag_t);
+                         ("data", cache_line_t);
+                         ("flag", enum_t MSI)] |}.
+
+  Definition ext_cache_mem_resp :=
+    {| struct_name := "ext_cache_mem_resp";
+       struct_fields := [("row", struct_t cache_row)] |}.
+
+  Definition cache_mem_output :=
+    {| struct_name := "cache_mem_output";
+       struct_fields := [("get_valid", bits_t 1);
+                        ("put_ready", bits_t 1);
+                        ("get_response", struct_t ext_cache_mem_resp)] |}.
+
+
+  Definition Sigma (fn: ext_fn_t) :=
+    match fn with
+    | ext_mem imem => {$ struct_t cache_mem_input ~> struct_t cache_mem_output $}
+    | ext_mem dmem => {$ struct_t cache_mem_input ~> struct_t cache_mem_output $}
+    | ext_mem mainmem => {$ struct_t mem_input ~> struct_t mem_output $}
     | ext_uart_read => {$ bits_t 1 ~> uart_output $}
     | ext_uart_write => {$ uart_input ~> bits_t 1 $}
     | ext_led => {$ led_input ~> bits_t 1 $}
